trunk/source/CoreRCP/src/de/uni_freiburg/informatik/ultimate/model/boogie/ast/BoogieASTNode.java
@@ -1,10 +1,17 @@
 package de.uni_freiburg.informatik.ultimate.model.boogie.ast;
 
+import java.util.ArrayList;
+import java.util.List;
+
 import de.uni_freiburg.informatik.ultimate.model.location.BoogieLocation;
 import de.uni_freiburg.informatik.ultimate.model.location.ILocation;
-import de.uni_freiburg.informatik.ultimate.model.structure.BaseSimpleAST;
+import de.uni_freiburg.informatik.ultimate.model.structure.BasePayloadContainer;
+import de.uni_freiburg.informatik.ultimate.model.structure.ISimpleAST;
+import de.uni_freiburg.informatik.ultimate.model.structure.IWalkable;
+import de.uni_freiburg.informatik.ultimate.model.structure.VisualizationNode;
 
-public class BoogieASTNode extends BaseSimpleAST<BoogieASTNode> {
+
+public class BoogieASTNode extends BasePayloadContainer implements ISimpleAST<BoogieASTNode>  {
 
 	private static final long serialVersionUID = 5856434889026482850L;
 
@@ -25,13 +32,32 @@ public class BoogieASTNode extends BaseSimpleAST<BoogieASTNode> {
 	protected BoogieASTNode createSpecialChild(String name, Object[] childs) {
 		BoogieASTWrapper parent = new BoogieASTWrapper(null, name);
 		for (Object obj : childs) {
-			parent.mOutgoingNodes.add(createSpecialChild(obj));
+			parent.getOutgoingNodes().add(createSpecialChild(obj));
 		}
 		return parent;
 	}
 
 	protected BoogieASTNode createSpecialChild(Object obj) {
 		return new BoogieASTWrapper(null, obj);
+	}
+	
+	@Override
+	public VisualizationNode getVisualizationGraph() {
+		return new VisualizationNode(this);
+	}
+
+	@Override
+	public List<IWalkable> getSuccessors() {
+		ArrayList<IWalkable> rtr = new ArrayList<>();
+		for(BoogieASTNode node : getOutgoingNodes()){
+			rtr.add(node);
+		}
+		return rtr;
+	}
+
+	@Override
+	public List<BoogieASTNode> getOutgoingNodes() {
+		return new ArrayList<BoogieASTNode>();
 	}
 
 	private class BoogieASTWrapper extends BoogieASTNode {
@@ -54,5 +80,4 @@ public class BoogieASTNode extends BaseSimpleAST<BoogieASTNode> {
 		}
 
 	}
-
 }
